Primitive_Matchers/Common_Primitive_toString.thy
@@ -19,6 +19,12 @@ definition ipv4_cidr_toString :: "(ipv4addr \<times> nat) \<Rightarrow> string" 
 
 lemma "ipv4_cidr_toString (ipv4addr_of_dotdecimal (192,168,0,1), 22) = ''192.168.0.1/22''" by eval
 
+
+fun ipv4addr_wordinterval_toString :: "32 wordinterval \<Rightarrow> string" where
+  "ipv4addr_wordinterval_toString (WordInterval s e) = (if s = e then ipv4addr_toString s else ''{''@ipv4addr_toString s@''..''@ipv4addr_toString e@''}'')" |
+  "ipv4addr_wordinterval_toString (RangeUnion a b) = ipv4addr_wordinterval_toString a @ '' u ''@ipv4addr_wordinterval_toString b"
+
+
 fun protocol_toString :: "protocol \<Rightarrow> string" where
   "protocol_toString (ProtoAny) = ''all''" |
   "protocol_toString (Proto TCP) = ''tcp''" |
