Semantics_Ternary/Unknown_Match_Tacs.thy
@@ -31,8 +31,15 @@ fun in_doubt_deny :: "'packet unknown_match_tac" where
 lemma wf_in_doubt_deny: "wf_unknown_match_tac in_doubt_deny"
   unfolding wf_unknown_match_tac_def by(simp add: fun_eq_iff)
 
-lemma packet_independent_unknown_match_tacs: "packet_independent_\<alpha> in_doubt_allow"
+lemma packet_independent_unknown_match_tacs:
+    "packet_independent_\<alpha> in_doubt_allow"
     "packet_independent_\<alpha> in_doubt_deny"
   by(simp_all add: packet_independent_\<alpha>_def)
+
+
+lemma Drop_neq_Accept_unknown_match_tacs:
+      "in_doubt_allow Drop \<noteq> in_doubt_allow Accept"
+      "in_doubt_deny Drop \<noteq> in_doubt_deny Accept"
+  by(simp_all add: fun_eq_iff)
 
 end
